src/Examples/Logging/LogicalLog.v
@@ -597,11 +597,11 @@ Inductive Recghost (restrict:LogicalState -> Prop) :=
 
 Arguments recghost {restrict}.
 
-Theorem log_apply_spec_idempotent_crash_step :
-  idempotent_crash_step
-                (fun '(ps, ls) => log_apply_spec ps ls ls.(ls_disk) ls.(ls_committed)).
+Theorem log_apply_spec_idempotent :
+  idempotent
+    (fun '(ps, ls) => log_apply_spec ps ls ls.(ls_disk) ls.(ls_committed)).
 Proof.
-  unfold idempotent_crash_step; intuition eauto; simplify.
+  unfold idempotent; intuition eauto; simplify.
   simpl in H0; propositional.
   destruct_with_eqn (b.(ls_committed)); split_cases;
     match goal with
@@ -614,18 +614,18 @@ Proof.
     simplify; finish.
 Qed.
 
-Theorem log_apply_spec_idempotent_crash_step' ls0 :
-  idempotent_crash_step
-                (fun (a: Recghost (fun ls =>
-                                   if ls.(ls_committed) then
-                                     massign ls.(ls_log) ls.(ls_disk) =
-                                     massign ls0.(ls_log) ls0.(ls_disk)
-                                   else ls.(ls_disk) = ls0.(ls_disk) \/
-                                        ls.(ls_disk) = massign ls0.(ls_log) ls0.(ls_disk))) =>
-                   let 'recghost ps ls _ := a in
-                   log_apply_spec ps ls ls.(ls_disk) ls.(ls_committed)).
+Theorem log_apply_spec_idempotent' ls0 :
+  idempotent
+    (fun (a: Recghost (fun ls =>
+                       if ls.(ls_committed) then
+                         massign ls.(ls_log) ls.(ls_disk) =
+                         massign ls0.(ls_log) ls0.(ls_disk)
+                       else ls.(ls_disk) = ls0.(ls_disk) \/
+                            ls.(ls_disk) = massign ls0.(ls_log) ls0.(ls_disk))) =>
+       let 'recghost ps ls _ := a in
+       log_apply_spec ps ls ls.(ls_disk) ls.(ls_committed)).
 Proof.
-  unfold idempotent_crash_step; intuition eauto; simplify.
+  unfold idempotent; intuition eauto; simplify.
   destruct a.
   simpl in *; propositional.
   destruct_with_eqn (ls.(ls_committed)); split_cases;
@@ -636,13 +636,13 @@ Proof.
     end; simpl; simplify; finish.
 Qed.
 
-Theorem log_apply_spec_idempotent_crash_step_notxn' ls0 :
-  idempotent_crash_step
-                (fun (a: Recghost (fun ls => ls.(ls_disk) = ls0.(ls_disk))) =>
-                   let 'recghost ps ls _ := a in
-                   log_apply_spec ps ls ls.(ls_disk) false).
+Theorem log_apply_spec_idempotent_notxn' ls0 :
+  idempotent
+    (fun (a: Recghost (fun ls => ls.(ls_disk) = ls0.(ls_disk))) =>
+       let 'recghost ps ls _ := a in
+       log_apply_spec ps ls ls.(ls_disk) false).
 Proof.
-  unfold idempotent_crash_step; intuition eauto; simplify.
+  unfold idempotent; intuition eauto; simplify.
   destruct a.
   simpl in H0; propositional.
   destruct_with_eqn (ls.(ls_committed)); split_cases;
