src/Examples/ReplicatedDisk/TwoDiskTheorems.v
@@ -14,17 +14,17 @@ Section specs.
      We use these exclusively in this file to prove higher level specs below. *)
   Lemma read_op_ok :
     forall i a,
-      proc_hspec TDBaseDynamics (td.read i a) (op_cstep_spec TDBaseDynamics (op_read i a)).
+      proc_hspec TDBaseDynamics (td.read i a) (op_spec TDBaseDynamics (op_read i a)).
   Proof. intros. eapply op_spec_sound. Qed.
 
   Lemma write_op_ok :
     forall i a b,
-      proc_hspec TDBaseDynamics (td.write i a b) (op_cstep_spec TDBaseDynamics (op_write i a b)).
+      proc_hspec TDBaseDynamics (td.write i a b) (op_spec TDBaseDynamics (op_write i a b)).
   Proof. intros. eapply op_spec_sound. Qed.
 
   Lemma size_op_ok :
     forall i,
-      proc_hspec TDBaseDynamics (td.size i) (op_cstep_spec TDBaseDynamics (op_size i)).
+      proc_hspec TDBaseDynamics (td.size i) (op_spec TDBaseDynamics (op_size i)).
   Proof. intros. eapply op_spec_sound. Qed.
 
   Hint Resolve read_op_ok : core.
